susp serialization library security (with some admitted cases)

theories/examples/authentikit_susp_security.v
@@ -4,27 +4,71 @@ From auth.heap_lang Require Import gen_weakestpre.
 From auth.heap_lang.lib Require Import list serialization.
 From auth.examples Require Export authentikit_susp authenticatable_base_susp.
 From iris.base_logic.lib Require Export invariants.
-
-Section auth_serialization.
+  
+(* Section auth_serialization.
   Context `{invGS_gen hlc Σ} `{g : !GenWp Σ} (N : namespace).
 
   Implicit Types c : gwp_type g.
 
+  Definition authSerBaseN : namespace := N .@ "auth_ser".
+  Definition authSerN (v : val) : namespace := N .@ v.
+
   Definition auth_valid_val (v : val) : iProp Σ :=
-    (∃ (h : string), ⌜v = InjLV #h⌝) ∨
+    ((∃ (h : string), ⌜v = InjLV #h⌝) ∨
       (∃ (susp : loc), ⌜v = InjRV #susp⌝ ∗
         ((∃ (h : string), gwp_pointsto g susp DfracDiscarded (InjRV #h)) ∨
-          (∃ (pid : nat), gwp_pointsto g susp (DfracOwn 1) (InjLV #pid)))).
+          (∃ (pid : nat), gwp_pointsto g susp (DfracOwn 1) (InjLV #pid))))).
 
   Definition auth_is_ser (v : val) (s : string) : iProp Σ :=
-    (∃ (h : string), ⌜v = InjLV #h⌝ ∗ s_is_ser (g:=g) auth_scheme (SOMEV #h) s) ∨
+    inv (authSerN v) ((∃ (h : string), ⌜v = InjLV #h⌝ ∗ s_is_ser (g:=g) auth_scheme (SOMEV #h) s) ∨
        (∃ (susp : loc), ⌜v = InjRV #susp⌝ ∗
          ((∃ (h : string), gwp_pointsto g susp DfracDiscarded (InjRV #h) ∗ s_is_ser (g:=g) auth_scheme (SOMEV #h) s) ∨
-            (∃ (pid : nat), gwp_pointsto g susp (DfracOwn 1) (InjLV #pid) ∗ s_is_ser (g:=g) auth_scheme NONEV s))).
+            (∃ (pid : nat), gwp_pointsto g susp (DfracOwn 1) (InjLV #pid) ∗ s_is_ser (g:=g) auth_scheme NONEV s)))).
 
+  Definition auth_is_ser' (s : string) : iProp Σ :=
+    ∃ (h : string), s_is_ser (g:=g) auth_scheme (SOMEV #h) s ∨
+       s_is_ser (g:=g) auth_scheme NONEV s.
+
+  Instance gwp_pointsto_persistent l v :
+    Persistent (gwp_pointsto g l DfracDiscarded v).
+  Proof. Admitted.
+
+  Instance gwp_pointsto_timeless l v :
+    Timeless (gwp_pointsto g l DfracDiscarded v).
+  Proof. Admitted.
+  
   Lemma auth_is_ser_inj v s1 s2 :
-    auth_is_ser v s1 -∗ auth_is_ser v s2 -∗ ⌜s1 = s2⌝.
+    auth_is_ser v s1 -∗ auth_is_ser v s2 ={⊤}=∗ ⌜s1 = s2⌝.
   Proof.
+    iIntros "#Hs1 #Hs2". 
+    iInv "Hs1" as "[>(%&%&#H1)|(%&>%&[(%&>#H1&>#Hser1)|(%&H1&>#Hser1)])]"; iModIntro.
+    - iSplitL.
+      { iLeft. iFrame "% #". }
+      iInv "Hs2" as "[>(%&%&#H2)|(%&>%&[(%&H2&>#Hser2)|H2])]"; iModIntro; simplify_eq.
+      iSplitL.
+      { iLeft. by iFrame "# %". }
+      simplify_eq. iApply s_is_ser_inj; by iFrame "#".
+    - iSplitL.
+      { iRight. iExists _. iFrame "%". iLeft. by iFrame "# ∗". }
+      iInv "Hs2" as "[>(%&%&#H2)|(%&>%&[(%&>#H2&>#Hser2)|(%&H2&>#Hser2)])]" "Hclose";
+        simplify_eq; last first.
+      + iPoseProof (gwp_pointsto_agree with "H1 H2") as "H". simplify_eq.
+        iMod "H" as "%". simplify_eq.
+      + iPoseProof (gwp_pointsto_agree with "H1 H2") as "%". simplify_eq.
+        iPoseProof (s_is_ser_inj with "Hser1 Hser2") as "%". simplify_eq.
+        iMod ("Hclose" with "[]") as "_".
+        { iRight. iExists _. iSplit; [done|]. iLeft. iFrame "#". }
+        done.
+    - iSplitL.
+      { iRight. iExists _. iSplit; [done|]. iRight. by iFrame. }
+      iInv "Hs2" as "[>(%&%&#H2)|(%&>%&[(%&>#H2&>#Hser2)|(%&H2&>#Hser2)])]" "Hclose";
+        simplify_eq.
+      + iPoseProof (gwp_pointsto_agree with "H1 H2") as "H". simplify_eq.
+        iMod "H" as "%". simplify_eq.
+      
+    
+    iModIntro. iFrame. iIntros "H2".
+    iInv "Hs1" as "[(% & % & Hs1)|(% & % & [(% & Hl1 & Hs1)|(% & Hl1 & %)])]".
     iIntros "[(% & % & Hs1)|(% & % & [(% & Hl1 & Hs1)|(% & Hl1 & %)])] [(% & % & Hs2)|(% & % & [(% & Hl2 & Hs2)|(% & Hl2 & %)])]"; simplify_eq.
     - iEval (simpl) in "Hs1 Hs2".
       by iApply (option_is_ser_inj with "[Hs1] [Hs2]").
@@ -37,15 +81,25 @@ Section auth_serialization.
   Qed.
 
   Lemma auth_is_ser_valid v s : auth_is_ser v s ⊢ auth_valid_val v.
-  Proof.
-    iIntros "[(% & % & Hs1)|(% & % & [(% & Hl1 & Hs1)|(% & Hl1 & %)])]".
+  Proof. Admitted.
+(*    iIntros "[(% & % & Hs1)|(% & % & [(% & Hl1 & Hs1)|(% & Hl1 & %)])]".
     - iLeft. iFrame "%".
     - iRight. iFrame "%".
       iLeft. iFrame.
     - iRight. iFrame "%".
       iRight. iFrame.
-  Qed.
+  Qed. *)
 
+  Lemma auth_is_ser_eq v s :
+    auth_is_ser v s -∗ auth_is_ser' s.
+  Proof. Admitted.
+(*    iIntros "[(%&->&#Hser)|(%&->&[(%&Ho&#Hser)|(%&Ho&#Hser)])]"; rewrite /auth_is_ser';
+      iPoseProof (s_is_ser_eq with "Hser") as "Hser'".
+    - iLeft. eauto.
+    - iLeft. eauto.
+    - iRight. eauto.
+  Qed. *)
+      
   Lemma auth_ser_spec E v c :
     G{{{ ▷?(gwp_laters g) auth_valid_val v }}}
       auth_ser_v v @ c; E
@@ -96,8 +150,10 @@ Program Definition auth_serialization : serialization :=
   {| s_valid_val := λ _ Σ, @auth_valid_val _ Σ;
     s_serializer := auth_ser_v;
     s_is_ser := λ _ _ Σ, @auth_is_ser _ _ Σ;
+    s_is_ser' := λ _ _ Σ, @auth_is_ser' _ _ Σ;
     s_is_ser_inj := λ _ Σ, @auth_is_ser_inj _ Σ;
     s_is_ser_valid := λ _ Σ, @auth_is_ser_valid _ Σ;
+    s_is_ser_eq := @auth_is_ser_eq;
     s_ser_spec := @auth_ser_spec; |}.
 
 Section auth_deserialization.
@@ -153,105 +209,184 @@ Program Definition auth_deserialization : deserialization :=
   {| s_deserializer := auth_deser_v;
     s_deser_sound := ;
     s_deser_complete := ;
-  |}.
-  
-  Definition equivalent (t : evi_type) (v1 : val) (v2 : val) : val :=
-    match t with
-    | tprod t1 t2 => 
-    | tsum t1 t2 =>
-        (match: val with
-           InjLV "lv" => InjLV (make_serializable "lv")
-         | InjRV "rv" => InjRV (make_serializable "rv"))%I
-    | tstring => v
-    | tint => v
-    | tauth =>
-        (
-        
-  Fixpoint s_is_ser' (t : evi_type) (v : val) (s : string) : iProp Σ :=
-    match t with
-    | tprod t1 t2 => prod_is_ser' v s (s_is_ser' t1) (s_is_ser' t2)
-    | tsum t1 t2 => sum_is_ser' v s (s_is_ser' t1) (s_is_ser' t2)
-    | tstring => string_is_ser v s
-    | tint => int_is_ser v s
-    | tauth =>
-        (∃ (h : string), ⌜v = InjLV #h⌝ ∗ s_is_ser (g := gwp_upto_bad) auth_serialization_scheme (InjRV #h) s) ∨
-          (∃ (susp : loc), ⌜v = InjRV #susp⌝ ∗
-            ((∃ (h : string), susp ↦ (InjRV #h) ∗ s_is_ser (g := gwp_upto_bad) auth_serialization_scheme (InjRV #h) s) ∨
-               (∃ (v : val), susp ↦ InjLV v)))
-    end.
+  |}. *)
 
+Section authenticatable.
+  Context `{!heapGS_gen hlc Σ}.           
+  
   Inductive evi_type : Type :=
   | tprod (t1 t2 : evi_type)
   | tsum (t1 t2 : evi_type)
+  | toption (t1 : evi_type)
   | tstring
   | tint
   | tauth.
 
+  Definition auth_is_ser_1 (v : val) (s : string) : iProp Σ :=
+    ∃ (h : string), ⌜v = InjLV #h⌝ ∗ s_is_ser (g:=gwp_upto_bad) auth_scheme (SOMEV #h) s.
+
+  Definition auth_is_ser_2 (v : val) (s : string) : iProp Σ :=
+    ∃ (susp : loc) (h : string),
+      ⌜v = InjRV #susp⌝ ∗ susp ↦{DfracDiscarded} (InjRV #h) ∗ s_is_ser (g:=gwp_upto_bad) auth_scheme (SOMEV #h) s.
+
+  Definition auth_is_ser_3 (v : val) (s : string) : iProp Σ :=
+    ∃ (susp : loc),
+      ⌜v = InjRV #susp⌝ ∗ s_is_ser (g:=gwp_upto_bad) auth_scheme NONEV s.
+
+  Definition auth_valid_val (v : val) : iProp Σ :=
+    ((∃ (h : string), ⌜v = InjLV #h⌝) ∨
+       (∃ (susp : loc),
+           ⌜v = InjRV #susp⌝ ∗
+             (∃ (h : string), susp ↦{DfracDiscarded} (InjRV #h) ∨
+                (∃ (pid : nat), susp ↦ (InjLV #pid))))).
+  
+  Fixpoint s_is_ser_ser (t : evi_type) (v : val) (s : string) : iProp Σ :=
+    match t with
+    | tprod t1 t2 => prod_is_ser' v s (s_is_ser_ser t1) (s_is_ser_ser t2)
+    | tsum t1 t2 => sum_is_ser' v s (s_is_ser_ser t1) (s_is_ser_ser t2)
+    | toption t1 => option_is_ser' v s (s_is_ser_ser t1)
+    | tstring => string_is_ser v s
+    | tint => int_is_ser v s
+    | tauth => auth_is_ser_1 v s ∨ auth_is_ser_2 v s
+    end.
+
+  Fixpoint s_is_ser_deser (t : evi_type) (v : val) (s : string) : iProp Σ :=
+    match t with
+    | tprod t1 t2 => prod_is_ser' v s (s_is_ser_deser t1) (s_is_ser_deser t2)
+    | tsum t1 t2 => sum_is_ser' v s (s_is_ser_deser t1) (s_is_ser_deser t2)
+    | toption t1 => option_is_ser' v s (s_is_ser_deser t1)
+    | tstring => string_is_ser v s
+    | tint => int_is_ser v s
+    | tauth => auth_is_ser_1 v s ∨ auth_is_ser_3 v s
+    end.
+
+  Fixpoint s_is_ser'' (t : evi_type) (v : val) (s : string) : iProp Σ :=
+    match t with
+    | tprod t1 t2 => prod_is_ser' v s (s_is_ser'' t1) (s_is_ser'' t2)
+    | tsum t1 t2 => sum_is_ser' v s (s_is_ser'' t1) (s_is_ser'' t2)
+    | toption t1 => option_is_ser' v s (s_is_ser'' t1)
+    | tstring => string_is_ser v s
+    | tint => int_is_ser v s
+    | tauth => auth_is_ser_1 v s ∨ auth_is_ser_2 v s ∨ auth_is_ser_3 v s
+    end.
+
+  #[global] Instance s_is_ser''_persistent t v s: Persistent (s_is_ser'' t v s).
+  Proof. Admitted.
+  
   #[global] Instance : Inhabited evi_type.
   Proof. constructor. apply tstring. Qed.
 
-  Fixpoint evi_type_ser (t : evi_type) : serialization_scheme :=
+  (* Fixpoint evi_type_ser (t : evi_type) : serialization_scheme :=
     match t with
     | tprod t1 t2 => prod_serialization_scheme (evi_type_ser t1) (evi_type_ser t2)
     | tsum t1 t2 => sum_serialization_scheme (evi_type_ser t1) (evi_type_ser t2)
     | tstring => string_serialization_scheme
     | tint => int_serialization_scheme
     | tauth => auth_serialization_scheme
-    end.
+    end. *)
   
   Fixpoint evi_type_count (t : evi_type) : expr :=
     match t with
     | tprod t1 t2 => prod_count (evi_type_count t1) (evi_type_count t2)
     | tsum t1 t2 => sum_count (evi_type_count t1) (evi_type_count t2)
+    | toption t1 => option_count (evi_type_count t1)
     | tstring => string_count
     | tint => int_count
     | tauth => auth_count
     end.
 
-  Fixpoint count_is_correct (t : evi_type) (v : val) (c : val) : iProp Σ :=
+  Fixpoint count_is_correct (t : evi_type) (v : val) (c : nat) :=
     match t with
     | tprod t1 t2 =>
         ∃ (c1 c2 : nat) (v1 v2 : val),
-          count_is_correct t1 v1 #c1 ∗ count_is_correct t2 v2 #c2 ∗ ⌜#(c1 + c2) = c⌝
+          v = (v1, v2)%V ∧ count_is_correct t1 v1 c1 ∧ count_is_correct t2 v2 c2 ∧ (c1 + c2) = c
     | tsum t1 t2 =>
-        (∃ (v1 : val), count_is_correct t1 v1 c) ∨ (∃ (v2 : val), count_is_correct t2 v2 c)
-    | tstring | tint => ⌜c = #0⌝                                                 
+        (∃ (v1 : val), v = InjLV v1 ∧ count_is_correct t1 v1 c) ∨
+          (∃ (v2 : val), v = InjRV v2 ∧ count_is_correct t2 v2 c)
+    | toption t1 =>
+        (v = NONEV ∧ c = 0) ∨ (∃ (v1 : val), v = SOMEV v1 ∧ count_is_correct t1 v1 c)
+    | tstring | tint => c = 0
     | tauth =>
-        (∃ (l : val), ⌜v = InjLV l ∧ c = #1⌝) ∨ (∃ (r : val), ⌜v = InjRV r ∧ c = #0⌝)
+        (∃ (l : val), v = InjLV l ∧ c = 1) ∨ (∃ (r : val), v = InjRV r ∧ c = 0)
     end.
                                                  
   Definition ser_spec (ser : val) (t : evi_type) (A : lrel Σ) : iProp Σ :=
     ∀ (v1 v2 : val),
-      {{{ ▷ A v1 v2 }}} ser v1 {{{ s, RET #s; s_is_ser (g := gwp_upto_bad) (evi_type_ser t) v1 s }}}.
+      {{{ ▷ A v1 v2 }}}
+        ser v1
+      {{{ s, RET #s; s_is_ser'' t v1 s }}}.
 
   Definition deser_spec (deser : val) (t : evi_type) : iProp Σ :=
-    ∀ (pid : nat) (s : string),
+    ∀ (pid : nat),
       {{{ True }}}
-        deser #pid #s
-        {{{ o, RET $o; if o is Some v then s_is_ser (g := gwp_upto_bad) (evi_type_ser t) v s else True }}}.
+      deser #pid
+      {{{ (deser_partial : val), RET deser_partial;
+          ∀ (s : string),
+            {{{ True }}}
+              deser_partial #s
+              {{{ o, RET $o; if o is Some v then s_is_ser_deser t v s else True }}}
+      }}}.
+  
+  Definition deser1_spec (deser_partial : val) (t : evi_type) : iProp Σ :=
+    ∀ (s : string),
+      ({{{ True }}}
+         deser_partial #s
+      {{{ o, RET $o; if o is Some v then s_is_ser_deser t v s else True }}}).
 
-  Definition count_spec (count : val) (t : evi_type) : iProp Σ :=
-    ∀ (v : val),
-      {{{ True }}}
-        count v
-        {{{ o, RET $o; if o is Some c then count_is_correct t v c else True }}}.
+  Definition count_spec (count : val) (t : evi_type) (A : lrel Σ): iProp Σ :=
+    ∀ (v1 v2 : val),
+      {{{ ▷ A v1 v2 }}}
+        count v1
+      {{{ v, RET v; ∃ (c : nat), ⌜v = #c ∧ count_is_correct t v1 c⌝ }}}.
 
   Definition lrel_evidence' (A : lrel Σ) : lrel Σ :=
     LRel (λ v1 v2,
         ∃ (t : evi_type) (ser deser count : val),
-          ⌜v1 = (ser, deser, count)%V⌝ ∗ ser_spec ser t A ∗ deser_spec deser t ∗ count_spec count t)%I.
+          ⌜v1 = (ser, deser, count)%V⌝ ∗ ser_spec ser t A ∗ count_spec count t A ∗
+            deser_spec deser t)%I.
 
   Program Definition lrel_evidence : kindO Σ (⋆ ⇒ ⋆)%kind := λne A, lrel_evidence' A.
   Next Obligation.
     intros ??????.
-    rewrite /lrel_car/= /ser_spec.
+    rewrite /lrel_car/= /ser_spec /count_spec.
     solve_proper.
+  Qed.
+
+  Lemma prod_ser'_spec_ser (HA HB : val → iProp Σ) (tA tB : evi_type) (serA serB v vA vB : val) :
+    (▷ ⌜v = (vA, vB)%V⌝) -∗
+    ({{{ ▷ HA vA }}}
+        serA vA
+      {{{ (s : string), RET #s; s_is_ser'' tA vA s }}}) -∗
+    ({{{ ▷ HB vB }}}
+        serB vB
+      {{{ (s : string), RET #s; s_is_ser'' tB vB s }}}) -∗
+    {{{ ▷ prod_valid_val' v HA HB }}}
+      prod_ser' serA serB v
+      {{{ (s : string), RET #s; prod_is_ser' v s (s_is_ser'' tA) (s_is_ser'' tB) }}}.
+  Proof.
+    iIntros "#Hv #HA #HB % !# Hp HΦ".
+    rewrite /prod_ser' /prod_is_ser.
+    wp_pures.
+    iDestruct "Hp" as (???) "[H1 H2]". iSimplifyEq.
+    wp_pures.
+    wp_apply ("HA" with "H1").
+    iIntros (s1) "Hs1".
+    wp_pures.
+    wp_apply ("HB" with "H2").
+    iIntros (s2) "Hs2".
+    wp_pures.
+    iApply "HΦ".
+    iModIntro.
+    iExists vA, vB, s1, s2; iSplit; auto.
   Qed.
   
 End authenticatable.
 
 Section proof.
-  Context `{!authG Σ}.
+  Context `{!authG Σ} (N : namespace).
+
+  Definition authSerBaseN : namespace := N .@ "auth_ser".
+  Definition authSerN (v : val) : namespace := N .@ v.
 
   Lemma refines_Auth_pair Θ (Δ : ctxO Σ Θ) :
     ⊢ ⟦ ∀: ⋆; ⋆, var2 var1 → var2 var0 → var2 (var1 * var0) ⟧
@@ -269,15 +404,15 @@ Section proof.
     iModIntro. iFrame.
     iIntros (??) "!# HA".
     interp_unfold! in "HA".
-    iDestruct "HA" as (tA serA deserA countA ->) "(#HserA & #HdeserA & #HcountA)". clear.
+    iDestruct "HA" as (tA serA deserA countA ->) "(#HserA & #HcountA & #HdeserA)". clear.
     iIntros (??) "Hi".
     i_pures; wp_pures.
     iModIntro. iFrame.
     iIntros (??) "!# HB".
     interp_unfold! in "HB".
-    iDestruct "HB" as (tB serB deserB countB ->) "(#HserB & #HdeserB & #HcountB)". clear.
+    iDestruct "HB" as (tB serB deserB countB ->) "(#HserB & #HcountB & #HdeserB)". clear.
     iIntros (??) "Hi".
-    i_pures; wp_pures.
+    i_pures; wp_pures. clear.
     rewrite /prod_scheme /prod_ser /prod_deser /prod_count.
     wp_pures. iFrame. iModIntro.
     interp_unfold!.
@@ -285,14 +420,213 @@ Section proof.
     iSplit; [done|]. clear. iSplit; [|iSplit].
     - iIntros (v1 v2 ?) "!# Hp H".
       iDestruct "Hp" as (w1 w2 u1 u2) "(>-> & >-> & #HA & #HB)".
-      wp_apply (prod_ser'_spec (evi_type_ser tA) (evi_type_ser tB)
-                  (λ v1, A v1 w2)%I (λ v1, B v1 u2)%I) => /=; [done| | | |done]. 
+      iSimpl in "H".
+      wp_apply (prod_ser'_spec_ser (λ v1, A v1 w2)%I (λ v1, B v1 u2)%I) => /=; [done| | | |done].  
       { iIntros (?) "!# _ H". by wp_apply ("HserA" with "HA"). }
       { iIntros (?) "!# _ H". by wp_apply ("HserB" with "HB"). }
-      iExists _, _.  eauto.
-    - iIntros (pid s Ψ) "!# _ HΨ". by wp_apply prod_deser'_sound.
+      iExists _, _. eauto.
+    - iIntros (???) "!# Hp HΨ".
+      iDestruct "Hp" as (w1 w2 u1 u2) "(>-> & >-> & #HA & #HB)".
+      wp_pures.
+      wp_apply "HcountB"; [done|].
+      iIntros (?) "(% & -> & %HcountB)".
+      wp_apply "HcountA"; [done|].
+      iIntros (?) "(% & -> & %HcountA)".
+      wp_pures. iModIntro.
+      iApply "HΨ".
+      iExists (c0+c).
+      iPureIntro. split.
+      { f_equal. by rewrite Nat2Z.inj_add. }
+      eexists _, _, _, _.
+      split; done.
+    - iIntros (pid ?) "!# _ HΨ".
+      wp_pures.
+      wp_apply "HdeserB"; [done|]. iIntros "%deparB #HdeparB".
+      wp_apply "HdeserA"; [done|]. iIntros "%deparA #HdeparA".
+      wp_pures. iModIntro. iApply "HΨ".
+      iIntros (s ?) "!# _ HΨ".
+      by wp_apply prod_deser'_sound.
   Qed.
   
+  Lemma refines_Auth_sum Θ (Δ : ctxO Σ Θ) :
+    ⊢ ⟦ ∀: ⋆; ⋆, var2 var1 → var2 var0 → var2 (var1 + var0) ⟧
+      (ext Δ lrel_evidence) v_Auth_sum i_Auth_sum.
+  Proof. Admitted.
+
+  Lemma refines_Auth_string :
+    ⊢ lrel_evidence lrel_string v_Auth_string i_Auth_string.
+  Proof. Admitted.
+
+  Lemma refines_Auth_int :
+    ⊢ lrel_evidence lrel_int v_Auth_int i_Auth_int.
+  Proof. Admitted.
+
+  Lemma refines_Auth_mu Θ (Δ : ctxO Σ Θ) :
+    ⊢ ⟦ ∀: ⋆ ⇒ ⋆, var1 (var0 (μ: ⋆; var1 var0)) → var1 (μ: ⋆; var1 var0) ⟧
+      (ext Δ lrel_evidence) v_Auth_mu i_Auth_mu.
+  Proof.
+    rewrite /lrel_car/=.
+    iIntros (A v1 v2) "!# _". iIntros (??) "Hi".
+    rewrite /i_Auth_mu /v_Auth_mu.
+    i_pures. wp_pures.
+    iFrame. iModIntro. clear.
+    interp_unfold!.
+    iIntros (??) "!# H".
+    iIntros (??) "Hi".
+    interp_unfold! in "H".
+    iDestruct "H" as "(%t & %ser & %deser & %count & -> & #Hser & #Hcount & #Hdeser)".
+    i_pures. wp_pures.
+    iFrame. iModIntro.
+    interp_unfold!.
+    iExists t, _, _, _. iSplit; [done|].
+    clear. iSplit; [|iSplit].
+    - iIntros (v1 v2 Ψ) "!# Hs HΨ".
+      wp_pures.
+      rewrite interp_rec_star_unfold.
+      rewrite interp_unseal /=.
+      by wp_apply ("Hser" with "Hs").
+    - iIntros (???) "!# #Hp HΨ". wp_pures.
+      rewrite interp_rec_star_unfold.
+      rewrite interp_unseal /=.
+      by iApply "Hcount".
+    - iIntros (pid Ψ) "!# _ HΨ". wp_pures.
+      iApply "HΨ". iModIntro.
+      iIntros (s ?) "!# _ HΨ". wp_pures.
+      wp_apply "Hdeser"; [done|].
+      iIntros (depar) "HΨ1".
+      by iApply "HΨ1".
+  Qed.
+
+  Definition lrel_auth' (A : lrel Σ) : lrel Σ :=
+    LRel (λ v1 v2,
+        (∃ (a1 : val) (t : evi_type) (s1 : string),
+            s_is_ser'' t a1 s1 ∗ A a1 v2 ∗ hashed s1 ∗
+              ⌜v1 = InjLV #(hash s1)⌝) ∨
+          (∃ (susp : loc),
+              ⌜v1 = InjRV #susp⌝ ∗
+                inv (authSerN #susp) ((∃ (a1 : val) (t : evi_type) (s1 : string),
+                    s_is_ser'' t a1 s1 ∗ A a1 v2 ∗ hashed s1 ∗
+                      susp ↦{DfracDiscarded} (InjRV #s1)) ∨
+                   (∃ (pid : nat), susp ↦ (InjLV #pid)))))%I.
+
+  
+  Program Definition lrel_auth : kindO Σ (⋆ ⇒ ⋆)%kind := λne A, lrel_auth' A.
+  Next Obligation. solve_proper. Qed.
+
+  Definition is_proof (v : val) : iProp Σ :=
+    ∃ (l : list string), ⌜is_list l v⌝.
+
+  Definition lrel_proof : lrel Σ :=
+    LRel (λ v1 _, is_proof v1 )%I.
+
+  Definition auth_ctx {Θ} (Δ : ctxO Σ Θ) (R : kindO Σ (⋆ ⇒ ⋆)) :=
+    ext (ext (ext Δ lrel_auth) R) lrel_evidence.
+
+  Lemma refines_Auth_auth Θ (Δ : ctxO Σ Θ) R :
+    ⊢ ⟦ ∀: ⋆, var1 (var3 var0) ⟧
+      (auth_ctx Δ R) v_Auth_auth i_Auth_auth.
+  Proof.
+    iIntros (A ??) "!# _"; rewrite -!/interp.
+    iIntros (??) "Hi".
+    rewrite /v_Auth_auth /i_Auth_auth.
+    i_pures; wp_pures.
+    iModIntro. iFrame.
+    rewrite /auth_ctx.
+    interp_unfold!.
+    iExists tauth, _, _, _.
+    iSplit; [done|]. clear. iSplit; [|iSplit].
+    - iIntros (???) "!# #Hauth H".
+      rewrite /auth_ser_v. wp_pure.
+      iDestruct "Hauth" as "[(%&%&%&Hser&HA&Hhash&%)|(%&%&Hinv)]";
+        simplify_eq; wp_pures.
+      + wp_apply s_ser_spec.
+        { iRight. eauto. }
+        iIntros (s) "Hser1".
+        iApply "H".
+        iLeft. iExists _. eauto.
+      + wp_bind (!_)%E.
+        iInv "Hinv" as "[(%&%&%&Hser&HA&Hhash&#Hsusp)|(%&Hsusp)]" "Hclose";
+          wp_load.
+        * iMod ("Hclose" with "[Hser HA Hhash Hsusp]") as "_".
+          { iLeft. iFrame "#∗". }
+          iModIntro. wp_pures.
+          wp_apply s_ser_spec.
+          { iRight. eauto. }
+          iIntros (s) "Hser1".
+          iApply "H".
+          iRight. iLeft. iExists _, _.
+          eauto.
+        * iMod ("Hclose" with "[Hsusp]") as "_".
+          { iRight. eauto. }
+          iModIntro. wp_pures.
+          wp_apply s_ser_spec.
+          { iLeft. eauto. }
+          iIntros (s) "Hser1".
+          iApply "H".
+          iRight. iRight. iExists _.
+          eauto.
+    - iIntros (???) "!# #Hauth H".
+      rewrite /auth_count. wp_pures.
+      iDestruct "Hauth" as "[(%&%&%&Hser&HA&Hhash&%)|(%&%&Hinv)]";
+        simplify_eq; wp_pures; iApply "H"; iModIntro.
+      + iExists 1. iPureIntro. split.
+        { f_equal. }
+        left. eauto.
+      + iExists 0. iPureIntro. split; [f_equal|].
+        right. eauto.
+    - iIntros (??) "!# _ H".
+      rewrite /auth_deser_v. wp_pures.
+      iModIntro. iApply "H".
+      iIntros (s?) "!# _ H".
+      wp_pures. wp_apply s_deser_sound; [done|].
+      iIntros ([] ?); wp_pures.
+      + destruct H as [(->&H)|(?&?&(->&H)&?)]; wp_pures.
+        * wp_alloc susp. wp_pures.
+          iApply ("H" $! (Some _)).
+          iModIntro. simpl.
+          iRight. rewrite /auth_is_ser_3.
+          iExists _. iSplit; [done|].
+          eauto.
+        * iModIntro. iApply ("H" $! (Some _)).
+          iLeft. rewrite /auth_is_ser_1.
+          destruct! H0. simplify_eq.          
+          iExists _. iSplit; [done|].
+          iRight. iExists _, _.
+          eauto.
+      + by iApply ("H" $! None).
+  Qed.
+
+  Lemma refines_auth_auth Θ (Δ : ctxO Σ Θ) R :
+    ⊢ ⟦ ∀: ⋆, var1 var0 → var0 → var3 var0 ⟧
+      (auth_ctx Δ R) v_auth i_auth.
+  Proof.
+    iIntros (???) "!# _"; rewrite -/interp.
+    iIntros (??) "Hi".
+    rewrite /v_auth  /i_auth.
+    i_pures; wp_pures.
+    iModIntro. iFrame. clear.
+    iIntros (??) "!# #HeviA".
+    rewrite /auth_ctx.
+    interp_unfold! in "HeviA".
+    iDestruct "HeviA" as (tA ser count deser ->) "(#Hser & #Hcount & #Hdeser)".
+    iIntros (??) "Hi".
+    i_pures; wp_pures.
+    iFrame.
+    interp_unfold.
+    iIntros "!> !>" (w1 w2) "#HA". clear.
+    iIntros (??) "Hi".
+    i_pures; wp_pures.
+    interp_unfold! in "HA".
+    wp_apply "Hser"; [done|].
+    iIntros (s1) "#Hs1".
+    wp_apply (wp_hash with "[$]"). iIntros "#Hh1".
+    wp_pures.
+    iFrame.
+    interp_unfold!.
+    iLeft.    
+    iExists _,_,_. 
+    by iFrame "# %".
+  Qed.
   
   
 
